Added a more general ADT refinement for refining mutator methods.

ADT.v
@@ -1,4 +1,5 @@
 Require Export Common Computation.
+Require Import Ensembles.
 
 Generalizable All Variables.
 Set Implicit Arguments.
@@ -15,6 +16,14 @@ Definition observerMethodType (Ty : Type) :=
   Ty    (* Initial model *)
   -> nat (* Actual argument*)
   -> Comp nat. (* Return value *)
+
+(** Correctness property for mutators: Mutators should maintain
+   representation invariants. **)
+Definition mutatorInv rep (repInv : Ensemble rep) mutIdx mutators :=
+  forall (idx : mutIdx) (r : rep) (n : nat),
+    repInv r -> computational_inv repInv (mutators idx r n).
+
+Arguments mutatorInv rep repInv mutIdx mutators /.
 
 (** Interface of an ADT *)
 Record ADT :=
@@ -37,7 +46,7 @@ Record ADT :=
     ObserverMethods : ObserverIndex -> observerMethodType Rep;
     (** Observer method implementations *)
 
-    MutatorMethodsInv : forall idx r n, RepInv r -> computational_inv RepInv (MutatorMethods idx r n)
+    MutatorMethodsInv : mutatorInv RepInv MutatorMethods
     (** Mutator methods maintain Representation Invariants **)
 
     (** We probably want some sort of observer method specs as well.
